Getting somewhere

sat.dfy
@@ -1,6 +1,7 @@
 include "util.dfy"
 
-//Provably correct SAT solver
+// Provably correct SAT solver
+// inspired by https://siddhartha-gadgil.github.io/automating-mathematics/posts/sat-solving/
 newtype Variable = int
 
 datatype Expression = 
@@ -32,6 +33,7 @@ function descendents(e: Expression) : (d: set<Expression>)
     ensures e !in d
     ensures children(e) <= d
     ensures forall i :: i in d ==> height(e) > height(i)
+    ensures forall i :: i in children(e) ==> descendents(i) < d
 {
     match e {
         case Constant(b) => {}
@@ -42,6 +44,31 @@ function descendents(e: Expression) : (d: set<Expression>)
         case Implies(a,b) => {a, b} + descendents(a) + descendents(b)
         case Equivalent(a,b) => {a, b} + descendents(a) + descendents(b)
     }
+}
+
+function child_descendents(e: Expression) : (cd_flat: set<Expression>)
+    ensures flatten(set i | i in children(e) :: descendents(i)) <= descendents(e)
+    ensures cd_flat == flatten(set i | i in children(e) :: descendents(i))
+{
+    child_descendents_helper(e, descendents(e))
+}
+
+function child_descendents_helper(e: Expression, d: set<Expression>) : (cd_flat: set<Expression>)
+    requires d == descendents(e)
+    ensures flatten(set i | i in children(e) :: descendents(i)) <= d
+    ensures cd_flat == flatten(set i | i in children(e) :: descendents(i))
+{
+    assert forall i :: i in children(e) ==> descendents(i) < d;
+    assert e !in d;
+
+    var cs := children(e);
+    assert forall i :: i in cs ==> descendents(i) < d;
+    assert cs == children(e);
+    var cd_flat := flatten(set i | i in cs :: descendents(i));
+    assert cd_flat == flatten(set i | i in children(e) :: descendents(i));
+    assert cd_flat + cs == d;
+    assert cd_flat <= d;
+    cd_flat
 }
 
 function height(e: Expression) : (h: int)
@@ -90,8 +117,9 @@ function height(e: Expression) : (h: int)
     }
 }
 
-function vars(e: Expression) : set<Variable>
+function vars(e: Expression) : (vs: set<Variable>)
     decreases e, height(e)
+    ensures forall i :: i in children(e) ==> vs >= vars(i)
 {
     match e {
         case Constant(b) => {}
@@ -103,6 +131,40 @@ function vars(e: Expression) : set<Variable>
         case Equivalent(a,b) => vars(a) + vars(b)
     }
 }
+/*
+function set_vars(s: set<Expression>) : (vs: set<Variable>)
+    ensures forall i :: i in s ==> vars(i) <= vs
+    ensures flatten(set i | i in s :: vars(i)) == vs
+{
+    flatten(set i | i in s :: vars(i))
+}
+
+lemma bigger_set_bigger_vars(a: set<Expression>, b: set<Expression>, av: set<Variable>, bv: set<Variable>)
+    requires a <= b
+    requires set_vars(a) == av && set_vars(b) == bv
+    ensures av <= bv
+{
+
+}
+/*
+
+lemma descendent_vars(e: Expression, vs: set<Variable>)
+    requires vars(e) == vs
+    decreases height(e)
+    //ensures forall i :: i in descendents(e) ==> vars(e) >= vars(i)
+{
+    assert forall i :: i in children(e) ==> vars(e) >= vars(i);
+    var cs := children(e);
+    var cds := flatten(set i | i in children(e) :: descendents(i));
+    var ds := descendents(e);
+    //assert cds < ds;
+
+    var cds_vs := set_vars(cds);
+    var ds_vs := set_vars(ds);
+
+}
+
+*/
 
 function eval(e: Expression, vs: map<Variable,bool>) : bool
     requires vs.Keys >= vars(e)
@@ -119,7 +181,7 @@ function eval(e: Expression, vs: map<Variable,bool>) : bool
     }
 }
 
-lemma demorgan(s: set<Expression>, vs: map<Variable,bool>)
+lemma demorgan1(s: set<Expression>, vs: map<Variable,bool>)
     requires forall i :: i in s ==> vs.Keys >= vars(i)
     ensures eval(Not(Or(s)), vs) == eval(And(set i | i in s :: Not(i)), vs)
 {
@@ -135,12 +197,20 @@ lemma demorgan(s: set<Expression>, vs: map<Variable,bool>)
     assert !(!forall i :: i in s ==> !eval(i, vs)) == (forall i :: i in s ==> eval(Not(i), vs));
 }
 
-lemma descendents_vars(e: Expression, vs: map<Variable,bool>)
-    requires vs.Keys >= vars(e)
-    ensures forall i :: i in descendents(e) ==> vars(e) >= vars(i)
-    ensures forall i :: i in descendents(e) ==> vs.Keys >= vars(i)
+lemma demorgan2(s: set<Expression>, vs: map<Variable,bool>)
+    requires forall i :: i in s ==> vs.Keys >= vars(i)
+    ensures eval(Not(And(s)), vs) == eval(Or(set i | i in s :: Not(i)), vs)
 {
-
+    var x := eval(Not(And(s)), vs);
+    var and := And(s);
+    assert eval(and, vs) == (!forall i :: i in s ==> !eval(i, vs));
+    assert x == !(!forall i :: i in s ==> !eval(i, vs));
+    
+    var y := eval(Or(set i | i in s :: Not(i)), vs);
+    var nots := set i | i in s :: Not(i);
+    assert y == eval(Or(nots), vs);
+    assert eval(Or(nots), vs) == (forall i :: i in nots ==> eval(i, vs));
+    assert !(!forall i :: i in s ==> !eval(i, vs)) == (forall i :: i in s ==> eval(Not(i), vs));
 }
 
 function method simplify_one(e: Expression, vs: map<Variable,bool>) : (out: Expression)
@@ -152,6 +222,7 @@ function method simplify_one(e: Expression, vs: map<Variable,bool>) : (out: Expr
         case Not(ee) =>
             match ee {
                 case Or(_) => false
+                case And(_) => false
                 case _ => true
             }
         case e => true
@@ -175,8 +246,12 @@ function method simplify_one(e: Expression, vs: map<Variable,bool>) : (out: Expr
             var out := match n {
                 case Or(s) =>
                     descendents_vars(e, vs);
-                    demorgan(s, vs);
+                    demorgan1(s, vs);
                     And(set i | i in s :: Not(i))
+                case And(s) =>
+                    descendents_vars(e, vs);
+                    demorgan2(s, vs);
+                    Or(set i | i in s :: Not(i))
                 case _ => e
             };
             assert eval(e, vs) == eval(out, vs);
@@ -185,122 +260,122 @@ function method simplify_one(e: Expression, vs: map<Variable,bool>) : (out: Expr
     }
 }
 
+predicate no_implies(e: Expression) {
+    forall i :: i in {e} + descendents(e) ==> match i {
+        case Implies(_,_) => false 
+        case e => true
+    }
+}
+
 function method simplify_implies(e: Expression, vs: map<Variable,bool>) : (out: Expression)
     requires vs.Keys >= vars(e)
     decreases e
-    // ensures forall i :: i in {out} + descendents(out) ==> match i {
-    //     case Implies(_,_) => false 
-    //     case e => true
-    // }
+    ensures no_implies(out)
     ensures vars(e) >= vars(out)
     ensures eval(e, vs) == eval(out, vs)
 {
     descendents_vars(e, vs);
     var out := match e {
-        case Constant(b) => e
-        case Var(v) => e
-        case Not(x) => Not(simplify_implies(x, vs))
-        case And(s) => And(set i | i in s :: simplify_implies(i, vs))
-        case Or(s) => Or(set i | i in s :: simplify_implies(i, vs))
-        case Implies(a,b) => Or({Not(simplify_implies(a, vs)), simplify_implies(b, vs)})
-        case Equivalent(a,b) => Equivalent(simplify_implies(a, vs), simplify_implies(b, vs))
+        case Constant(b) =>
+            assert no_implies(e);
+            e
+        case Var(v) =>
+            assert no_implies(e);
+            e
+        case Not(x) => 
+            var xx := simplify_implies(x, vs);
+            assert no_implies(xx);
+            assert no_implies(Not(xx));
+            Not(xx)
+        case And(s) => 
+            var ss := set i | i in s :: simplify_implies(i, vs);
+            assert forall i :: i in ss ==> no_implies(i);
+            assert no_implies(And(ss));
+            And(ss)
+        case Or(s) =>
+            var ss := set i | i in s :: simplify_implies(i, vs);
+            assert forall i :: i in ss ==> no_implies(i);
+            assert no_implies(Or(ss));
+            Or(ss)
+        case Implies(a,b) => 
+            var a:= simplify_implies(a, vs);
+            assert no_implies(a) && no_implies(Not(a));
+            var b := simplify_implies(b, vs);
+            assert no_implies(b);
+            assert no_implies(Or({Not(a), b}));
+            Or({Not(a), b})
+        case Equivalent(a,b) => 
+            var a:= simplify_implies(a, vs);
+            assert no_implies(a);
+            var b := simplify_implies(b, vs);
+            assert no_implies(b);
+            assert no_implies(Equivalent(a, b));
+            Equivalent(a, b)
     };
-    assert match out {
-        case Implies(_,_) => false 
-        case e => true
-    };
-    assert forall i :: i in children(out) ==> match i {
-        case Implies(_,_) => false 
-        case e => true
-    };
-
-    // assert forall i :: i in descendents(out) ==> match i {
-    //     case Implies(_,_) => false 
-    //     case e => true
-    // };
 
     out
 }
 
-/*
-function method simplify_recurse(e: Expression, vs: map<Variable,bool>) : (out: Expression)
-    requires vs.Keys >= vars(e)
-    decreases e
-    ensures forall i :: i in {out} + children(out) ==> match i {
-        case Implies(_,_) => false 
-        case Equivalent(_,_) => false
-        case Not(ee) =>
-            match ee {
-                case Or(_) => false
-                case _ => true
-            }
+predicate no_equivalent(e: Expression) {
+    forall i :: i in {e} + descendents(e) ==> match i {
+        case Equivalent(_,_) => false 
         case e => true
     }
+}
+
+function method simplify_equivalent(e: Expression, vs: map<Variable,bool>) : (out: Expression)
+    requires vs.Keys >= vars(e)
+    ensures no_implies(e)
+    decreases e
+    ensures no_equivalent(out)
     ensures vars(e) >= vars(out)
     ensures eval(e, vs) == eval(out, vs)
 {
     descendents_vars(e, vs);
     var out := match e {
-        case Constant(b) => e
-        case Var(v) => e
-        case Not(x) => Not(simplify_recurse(x, vs))
-        case And(s) => And(set i | i in s :: simplify_recurse(i, vs))
-        case Or(s) => Or(set i | i in s :: simplify_recurse(i, vs))
-        case Implies(a,b) => Implies(simplify_recurse(a, vs), simplify_recurse(b, vs))
-        case Equivalent(a,b) => Equivalent(simplify_recurse(a, vs), simplify_recurse(b, vs))
-    };
-
-    assert forall i :: i in children(out) ==> match i {
-        case Implies(_,_) => false 
-        case Equivalent(_,_) => false
-        case Not(ee) =>
-            match ee {
-                case Or(_) => false
-                case _ => true
-            }
-        case e => true
-    };
-
-    assert vars(e) >= vars(out);
-    assert eval(e, vs) == eval(out, vs);
-    var out := simplify_one(out, vs);
-
-    assert match out {
-        case Implies(_,_) => false 
-        case Equivalent(_,_) => false
-        case Not(ee) =>
-            match ee {
-                case Or(_) => false
-                case _ => true
-            }
-        case e => true
-    };
-
-    var out := match out {
-        case Constant(b) => out
-        case Var(v) => out
-        case Not(x) => Not(simplify_recurse(x, vs))
-        case And(s) => And(set i | i in s :: simplify_recurse(i, vs))
-        case Or(s) => Or(set i | i in s :: simplify_recurse(i, vs))
-        case Implies(a,b) =>
+        case Constant(b) =>
+            assert no_equivalent(e);
+            e
+        case Var(v) =>
+            assert no_equivalent(e);
+            e
+        case Not(x) => 
+            var xx := simplify_equivalent(x, vs);
+            assert no_equivalent(xx);
+            assert no_equivalent(Not(xx));
+            Not(xx)
+        case And(s) => 
+            var ss := set i | i in s :: simplify_equivalent(i, vs);
+            assert forall i :: i in ss ==> no_equivalent(i);
+            assert no_equivalent(And(ss));
+            And(ss)
+        case Or(s) =>
+            var ss := set i | i in s :: simplify_equivalent(i, vs);
+            assert forall i :: i in ss ==> no_equivalent(i);
+            assert no_equivalent(Or(ss));
+            Or(ss)
+        case Implies(a,b) => 
             assert false;
-            out
+            a
         case Equivalent(a,b) => 
-            assert false;
+            var a:= simplify_equivalent(a, vs);
+            assert no_equivalent(a);
+            var b := simplify_equivalent(b, vs);
+            assert no_equivalent(b);
+            var out := Or(And({a,b}),And({Not(a),Not(b)}));
+            assert no_implies(out);
             out
-    };
-
-    assert forall i :: i in children(out) ==> match i {
-        case Implies(_,_) => false 
-        case Equivalent(_,_) => false
-        case Not(ee) =>
-            match ee {
-                case Or(_) => false
-                case _ => true
-            }
-        case e => true
     };
 
     out
 }
-*/
+
+function method simplify(e: Expression, vs: map<Variable,bool>) : (out: Expression)
+    requires vs.Keys >= vars(e)
+    ensures no_implies(out)
+    ensures no_equivalent(out)
+{
+    var out := simplify_implies(e, vs);
+    var out := simplify_equivalent(e, vs);
+    out
+}
